Evaluate.thy
@@ -6,7 +6,7 @@ inductive reduce :: "expr \<Rightarrow> expr \<Rightarrow> bool" (infix "\<leads
   ev_beta [simp]: "is_value e\<^sub>2 \<Longrightarrow> App (Abs t e\<^sub>1) e\<^sub>2 \<leadsto>\<^sub>\<beta> subst\<^sub>e\<^sub>e 0 e\<^sub>2 e\<^sub>1" 
 | ev_let [simp]: "is_value e\<^sub>1 \<Longrightarrow> Let e\<^sub>1 e\<^sub>2 \<leadsto>\<^sub>\<beta> subst\<^sub>e\<^sub>e 0 e\<^sub>1 e\<^sub>2"
 | ev_proj [simp]: "is_value_f fs \<Longrightarrow> lookup l fs = Some e \<Longrightarrow> Proj (Rec fs) l \<leadsto>\<^sub>\<beta> e" 
-| ev_case [simp]: "is_value e \<Longrightarrow> lookup l cs = Some e' \<Longrightarrow> Case (Inj l ts e) cs \<leadsto>\<^sub>\<beta> subst\<^sub>e\<^sub>e 0 e e'" 
+| ev_case [simp]: "is_value e \<Longrightarrow> lookup l cs = Some e' \<Longrightarrow> Case (Inj l ts e) t cs \<leadsto>\<^sub>\<beta> subst\<^sub>e\<^sub>e 0 e e'" 
 | ev_fold [simp]: "is_value e \<Longrightarrow> Unfold t (Fold t e) \<leadsto>\<^sub>\<beta> e" 
 | ev_tbeta [simp]: "TyApp (TyAbs e) t \<leadsto>\<^sub>\<beta> subst\<^sub>t\<^sub>e 0 t e" 
 | ev_tlet [simp]: "TyLet t e \<leadsto>\<^sub>\<beta> subst\<^sub>t\<^sub>e 0 t e" 
@@ -54,7 +54,7 @@ theorem [simp]: "\<Delta>,[] \<turnstile> e : t \<Longrightarrow> unfold e = (s,
     thus ?case
       proof (cases "is_value e")
       case True
-        with tc_case obtain l e' where E: "r = Case (Inj l ts e') cs \<and> is_value e' \<and> l < length ts" 
+        with tc_case obtain l e' where E: "r = Case (Inj l ts e') t cs \<and> is_value e' \<and> l < length ts" 
           by fastforce
         moreover with tc_case obtain r' where "lookup l cs = Some r'" by fastforce
         ultimately show ?thesis using ev_case by blast
@@ -96,8 +96,9 @@ theorem progress: "\<Delta>,[] \<turnstile> e : t \<Longrightarrow> is_value e \
 
 lemma preservation\<^sub>\<beta>: "e \<leadsto>\<^sub>\<beta> e' \<Longrightarrow> \<Delta>,\<Gamma> \<turnstile> e : t \<Longrightarrow> \<Delta>,\<Gamma> \<turnstile> e' : t"
   proof (induction e e' rule: reduce.induct) 
-  case (ev_case e l cs e' ts)
-    then obtain t' where "(\<Delta>,\<Gamma> \<turnstile> e : t') \<and> lookup l ts = Some t' \<and> \<Delta>,\<Gamma> \<turnstile>\<^sub>c cs : ts \<rightarrow> t" by fastforce
+  case (ev_case e l cs e' ts tt)
+    then obtain t' where "(\<Delta>,\<Gamma> \<turnstile> e : t') \<and> lookup l ts = Some t' \<and> (\<forall>tt \<in> set ts. \<Delta> \<turnstile>\<^sub>k tt) \<and> 
+      (\<Delta>,\<Gamma> \<turnstile>\<^sub>c cs : ts \<rightarrow> t) \<and> t = tt" by fastforce
     moreover with ev_case have "\<Delta>,insert_at 0 t' \<Gamma> \<turnstile> e' : t" by fastforce
     ultimately show ?case by simp
   next case (ev_tbeta e t')
